.

theories/Fol/Syntax.v
@@ -64,14 +64,12 @@ Fixpoint gen_trm (seed : nat) (d : nat) {struct d} : trm :=
   match d with
   | O => Var_trm seed
   | S d' =>
-    let seed1 := fst (cp seed) in
-    let seed' := snd (cp seed) in
-    let seed2 := fst (cp seed') in
-    let seed3 := snd (cp seed') in
+    let '(seed1, seed') := cp seed in
+    let '(seed2, seed3) := cp seed' in
     match seed1 with
     | 0 => Con_trm (enum_constant_symbols seed')
     | 1 => Fun_trm (enum_function_symbols seed2) (gen_trms seed3 d')
-    | S (S i) => Var_trm i
+    | S (S i) => (Var_trm i)
     end
   end
 with gen_trms {n : arity} (seed : nat) (d : nat) {struct d} : trms n :=
@@ -79,11 +77,10 @@ with gen_trms {n : arity} (seed : nat) (d : nat) {struct d} : trms n :=
   | O => O_trms
   | S n' =>
     match d with
-    | O => nat_rec _ (O_trms) (fun x => fun acc => S_trms _ (Var_trm seed) acc) (S n')
+    | O => nat_rec trms O_trms (fun m : nat => S_trms m (Var_trm seed)) (S n')
     | S d' =>
-      let seed1 := fst (cp seed) in
-      let seed2 := snd (cp seed) in
-      S_trms _ (gen_trm seed1 d') (gen_trms seed2 d')
+      let '(seed1, seed2) := cp seed in
+      S_trms n' (gen_trm seed1 d') (gen_trms seed2 d')
     end
   end.
 
@@ -99,29 +96,114 @@ Definition enum_trms {n : arity} (seed : nat) : trms n :=
 
 Section PROOF1.
 
+Lemma gen_trm_unfold (seed : nat) (d : nat) :
+  gen_trm seed d =
+  match d with
+  | O => Var_trm seed
+  | S d' =>
+    let '(seed1, seed') := cp seed in
+    let '(seed2, seed3) := cp seed' in
+    match seed1 with
+    | 0 => Con_trm (enum_constant_symbols seed')
+    | 1 => Fun_trm (enum_function_symbols seed2) (gen_trms seed3 d')
+    | S (S i) => (Var_trm i)
+    end
+  end.
+Proof. destruct d; reflexivity. Defined.
+
+Lemma gen_trms_unfold (n : arity) (seed : nat) (d : nat) :
+  gen_trms seed d =
+  match n with
+  | O => O_trms
+  | S n' =>
+    match d with
+    | O => nat_rec trms O_trms (fun m : nat => S_trms m (Var_trm seed)) (S n')
+    | S d' =>
+      let '(seed1, seed2) := cp seed in
+      S_trms n' (gen_trm seed1 d') (gen_trms seed2 d')
+    end
+  end.
+Proof. destruct d, n; reflexivity. Defined.
+
 Hypothesis enum_function_symbols_onto : forall f : L.(function_symbols), { n : nat | enum_function_symbols n = f }.
 Hypothesis enum_constant_symbols_onto : forall c : L.(constant_symbols), { n : nat | enum_constant_symbols n = c }.
+
+Lemma gen_trm_spec (t : trm) (d : nat)
+  (LE : trm_depth t <= d)
+  : { seed : nat | gen_trm seed d = t }
+with gen_trms_spec (n : arity) (ts : trms n) (d : nat)
+  (LE : trms_depth ts <= d)
+  : { seed : nat | gen_trms seed d = ts }.
+Proof.
+  - revert d LE. induction t as [x | f ts | c]; simpl; i.
+    + destruct d as [ | d'].
+      * exists x. reflexivity.
+      * simpl. exists (cpInv (2 + x) 0).
+        destruct (cp (cpInv (2 + x) 0)) as [x1 x2] eqn: H_OBS.
+        rewrite cp_spec in H_OBS. apply cpInv_inj in H_OBS. destruct H_OBS as [<- <-].
+        simpl. reflexivity.
+    + destruct d as [ | d']; [lia | assert (LE' : trms_depth ts <= d') by lia].
+      pose proof (gen_trms_spec _ ts d' LE') as [seed2 H_OBS].
+      exists (cpInv 1 (cpInv (proj1_sig (enum_function_symbols_onto f)) seed2)). rewrite gen_trm_unfold.
+      destruct (cp (cpInv 1 (cpInv (proj1_sig (enum_function_symbols_onto f)) seed2))) as [x1 x2] eqn: H_OBS'.
+      rewrite cp_spec in H_OBS'. apply cpInv_inj in H_OBS'. destruct H_OBS' as [<- <-].
+      destruct (cp (cpInv (proj1_sig (enum_function_symbols_onto f)) seed2)) as [x2 y2] eqn: H_OBS''.
+      rewrite cp_spec in H_OBS''. apply cpInv_inj in H_OBS''. destruct H_OBS'' as [<- <-].
+      assert (claim : enum_function_symbols (proj1_sig (enum_function_symbols_onto f)) = f) by now destruct (enum_function_symbols_onto f).
+      rewrite claim. rewrite H_OBS. reflexivity.
+    + destruct d as [ | d']; [lia | assert (LE' : 0 <= d') by lia].
+      exists (cpInv 0 (proj1_sig (enum_constant_symbols_onto c))). rewrite gen_trm_unfold.
+      destruct (cp (cpInv 0 (proj1_sig (enum_constant_symbols_onto c)))) as [x1 x2] eqn: H_OBS'.
+      assert (claim: enum_constant_symbols (proj1_sig (enum_constant_symbols_onto c)) = c) by now destruct (enum_constant_symbols_onto c).
+      rewrite cp_spec in H_OBS'. apply cpInv_inj in H_OBS'. destruct H_OBS' as [<- <-]. rewrite claim.
+      destruct (cp (proj1_sig (enum_constant_symbols_onto c))) as [x1 x2] eqn: H_OBS'. reflexivity.
+  - revert d LE. induction ts as [ | n t ts IH]; simpl; i.
+    + simpl. exists 0. rewrite gen_trms_unfold. reflexivity.
+    + destruct d as [ | d'].
+      * lia.
+      * assert (claim1 : trm_depth t <= d') by lia.
+        assert (claim2 : trms_depth ts <= d') by lia.
+        apply gen_trm_spec in claim1. apply IH in claim2.
+        destruct claim1 as [seed1 P_t'], claim2 as [seed2 P_ts'].
+        exists (cpInv seed1 seed2). rewrite <- P_t' at 1; rewrite <- P_ts' at 1. rewrite gen_trms_unfold.
+        destruct (cp (cpInv seed1 seed2)) as [x y] eqn: H_OBS. rewrite cp_spec in H_OBS.
+        apply cpInv_inj in H_OBS. destruct H_OBS as [<- <-]. reflexivity.
+Qed.
+
+Theorem enum_trm_spec (t : trm)
+  : { seed : nat | enum_trm seed = t }.
+Proof.
+  epose proof (gen_trm_spec t (trm_depth t) _) as [seed H_EQ].
+  exists (cpInv (trm_depth t) seed). unfold enum_trm. destruct (cp (cpInv (trm_depth t) seed)) as [x y] eqn: H_OBS.
+  rewrite cp_spec in H_OBS. apply cpInv_inj in H_OBS. destruct H_OBS as [<- <-]. simpl. done.
+  Unshelve. reflexivity.
+Qed.
+
+Theorem enum_trms_spec (n : arity) (ts : trms n)
+  : { seed : nat | enum_trms seed = ts }.
+Proof.
+  epose proof (gen_trms_spec n ts (trms_depth ts) _) as [seed H_EQ].
+  exists (cpInv (trms_depth ts) seed). unfold enum_trms. destruct (cp (cpInv (trms_depth ts) seed)) as [x y] eqn: H_OBS.
+  rewrite cp_spec in H_OBS. apply cpInv_inj in H_OBS. destruct H_OBS as [<- <-]. simpl. done.
+  Unshelve. reflexivity.
+Qed.
 
 End PROOF1.
 
 Variable enum_relation_symbols : nat -> L.(relation_symbols).
 
-Fixpoint gen_frm (seed: nat) (d: nat) {struct d} : frm :=
+Fixpoint gen_frm (seed : nat) (d : nat) {struct d} : frm :=
   match d with
   | O =>
-    let seed1 := fst (cp seed) in
-    let seed' := snd (cp seed) in
-    let seed2 := fst (cp seed') in
-    let seed3 := snd (cp seed') in
+    let '(seed1, seed') := cp seed in
+    let '(seed2, seed3) := cp seed' in
     match seed1 with
     | 0 => Eqn_frm (enum_trm seed2) (enum_trm seed3)
     | _ => Rel_frm (enum_relation_symbols seed2) (enum_trms seed3)
     end
   | S d' =>
-    let seed1 := fst (cp seed) in
-    let seed' := snd (cp seed) in
-    let seed2 := fst (cp seed') in
-    let seed3 := snd (cp seed') in
+    let '(seed1, seed') := cp seed in
+    let '(seed2, seed3) := cp seed' in
     match seed1 with
     | 0 => Neg_frm (gen_frm seed' d')
     | 1 => Imp_frm (gen_frm seed2 d') (gen_frm seed3 d')
@@ -141,13 +223,129 @@ Definition enum_frm (seed : nat) : frm :=
 
 Section PROOF2.
 
+Lemma gen_frm_unfold (seed : nat) (d : nat) :
+  gen_frm seed d =
+  match d with
+  | O =>
+    let '(seed1, seed') := cp seed in
+    let '(seed2, seed3) := cp seed' in
+    match seed1 with
+    | 0 => Eqn_frm (enum_trm seed2) (enum_trm seed3)
+    | _ => Rel_frm (enum_relation_symbols seed2) (enum_trms seed3)
+    end
+  | S d' =>
+    let '(seed1, seed') := cp seed in
+    let '(seed2, seed3) := cp seed' in
+    match seed1 with
+    | 0 => Neg_frm (gen_frm seed' d')
+    | 1 => Imp_frm (gen_frm seed2 d') (gen_frm seed3 d')
+    | 2 => All_frm seed2 (gen_frm seed3 d')
+    | S (S (S i)) =>
+      match i with
+      | 0 => Eqn_frm (enum_trm seed2) (enum_trm seed3)
+      | _ => Rel_frm (enum_relation_symbols seed2) (enum_trms seed3)
+      end
+    end
+  end.
+Proof. destruct d; reflexivity. Defined.
+
 Hypothesis enum_function_symbols_onto : forall f : L.(function_symbols), { n : nat | enum_function_symbols n = f }.
 Hypothesis enum_constant_symbols_onto : forall c : L.(constant_symbols), { n : nat | enum_constant_symbols n = c }.
 Hypothesis enum_relation_symbols_onto : forall R : L.(relation_symbols), { n : nat | enum_relation_symbols n = R }.
 
+Lemma gen_frm_spec (p : frm) (d : nat)
+  (LE : frm_depth p <= d)
+  : { seed : nat | gen_frm seed d = p }.
+Proof.
+  revert d LE. induction p as [R ts | t1 t2 | p1 IH1 | p1 IH1 p2 IH2 | y p1 IH1]; simpl; i.
+  - destruct d as [ | d'].
+    + exists (cpInv 1 (cpInv (proj1_sig (enum_relation_symbols_onto R)) (proj1_sig (enum_trms_spec enum_function_symbols_onto enum_constant_symbols_onto _ ts)))).
+      rewrite gen_frm_unfold. destruct (cp (cpInv 1 (cpInv (proj1_sig (enum_relation_symbols_onto R)) (proj1_sig _)))) as [x y] eqn: H_OBS.
+      rewrite cp_spec in H_OBS. apply cpInv_inj in H_OBS. destruct H_OBS as [<- <-].
+      destruct (cp (cpInv (proj1_sig (enum_relation_symbols_onto R)) (proj1_sig _))) as [x y] eqn: H_OBS.
+      rewrite cp_spec in H_OBS. apply cpInv_inj in H_OBS. destruct H_OBS as [<- <-].
+      destruct (enum_relation_symbols_onto R) as [R_n H_R], (enum_trms_spec enum_function_symbols_onto enum_constant_symbols_onto _ ts) as [ts_n H_ts]; subst R ts. reflexivity.
+    + exists (cpInv 4 (cpInv (proj1_sig (enum_relation_symbols_onto R)) (proj1_sig (enum_trms_spec enum_function_symbols_onto enum_constant_symbols_onto _ ts)))).
+      rewrite gen_frm_unfold. destruct (cp (cpInv 4 (cpInv (proj1_sig (enum_relation_symbols_onto R)) (proj1_sig _)))) as [x y] eqn: H_OBS.
+      rewrite cp_spec in H_OBS. apply cpInv_inj in H_OBS. destruct H_OBS as [<- <-].
+      destruct (cp (cpInv (proj1_sig (enum_relation_symbols_onto R)) (proj1_sig _))) as [x y] eqn: H_OBS.
+      rewrite cp_spec in H_OBS. apply cpInv_inj in H_OBS. destruct H_OBS as [<- <-].
+      destruct (enum_relation_symbols_onto R) as [R_n H_R], (enum_trms_spec enum_function_symbols_onto enum_constant_symbols_onto _ ts) as [ts_n H_ts]; subst R ts. reflexivity.
+  - destruct d as [ | d'].
+    + exists (cpInv 0 (cpInv (proj1_sig (enum_trm_spec enum_function_symbols_onto enum_constant_symbols_onto t1)) (proj1_sig (enum_trm_spec enum_function_symbols_onto enum_constant_symbols_onto t2)))).
+      rewrite gen_frm_unfold. destruct (cp (cpInv 0 (cpInv (proj1_sig _) (proj1_sig _)))) as [x y] eqn: H_OBS.
+      rewrite cp_spec in H_OBS. apply cpInv_inj in H_OBS. destruct H_OBS as [<- <-].
+      destruct (cp (cpInv (proj1_sig _) (proj1_sig _))) as [x y] eqn: H_OBS.
+      rewrite cp_spec in H_OBS. apply cpInv_inj in H_OBS. destruct H_OBS as [<- <-].
+      destruct (enum_trm_spec enum_function_symbols_onto enum_constant_symbols_onto t1) as [t1_n H_t1], (enum_trm_spec enum_function_symbols_onto enum_constant_symbols_onto t2) as [t2_n H_t2]; subst t1 t2. reflexivity.
+    + exists (cpInv 3 (cpInv (proj1_sig (enum_trm_spec enum_function_symbols_onto enum_constant_symbols_onto t1)) (proj1_sig (enum_trm_spec enum_function_symbols_onto enum_constant_symbols_onto t2)))).
+      rewrite gen_frm_unfold. destruct (cp (cpInv 3 (cpInv (proj1_sig _) (proj1_sig _)))) as [x y] eqn: H_OBS.
+      rewrite cp_spec in H_OBS. apply cpInv_inj in H_OBS. destruct H_OBS as [<- <-].
+      destruct (cp (cpInv (proj1_sig _) (proj1_sig _))) as [x y] eqn: H_OBS.
+      rewrite cp_spec in H_OBS. apply cpInv_inj in H_OBS. destruct H_OBS as [<- <-].
+      destruct (enum_trm_spec enum_function_symbols_onto enum_constant_symbols_onto t1) as [t1_n H_t1], (enum_trm_spec enum_function_symbols_onto enum_constant_symbols_onto t2) as [t2_n H_t2]; subst t1 t2. reflexivity.
+  - destruct d as [ | d'].
+    + lia.
+    + assert (claim1 : frm_depth p1 <= d') by lia.
+      apply IH1 in claim1. destruct claim1 as [seed1 H_seed1]. exists (cpInv 0 seed1).
+      rewrite gen_frm_unfold. destruct (cp (cpInv 0 seed1)) as [x y] eqn: H_OBS.
+      rewrite cp_spec in H_OBS. apply cpInv_inj in H_OBS. destruct H_OBS as [<- <-].
+      destruct (cp seed1) as [x y]. congruence.
+  - destruct d as [ | d'].
+    + lia.
+    + assert (claim1 : frm_depth p1 <= d') by lia.
+      assert (claim2 : frm_depth p2 <= d') by lia.
+      apply IH1 in claim1. apply IH2 in claim2. destruct claim1 as [seed1 H_seed1]. destruct claim2 as [seed2 H_seed2]. exists (cpInv 1 (cpInv seed1 seed2)).
+      rewrite gen_frm_unfold. destruct (cp (cpInv 1 (cpInv seed1 seed2))) as [x y] eqn: H_OBS.
+      rewrite cp_spec in H_OBS. apply cpInv_inj in H_OBS. destruct H_OBS as [<- <-].
+      destruct (cp (cpInv seed1 seed2)) as [x y] eqn: H_OBS. rewrite cp_spec in H_OBS. apply cpInv_inj in H_OBS. destruct H_OBS as [<- <-]. congruence.
+  - destruct d as [ | d'].
+    + lia.
+    + assert (claim1 : frm_depth p1 <= d') by lia.
+      apply IH1 in claim1. destruct claim1 as [seed1 H_seed1]. exists (cpInv 2 (cpInv y seed1)).
+      rewrite gen_frm_unfold. destruct (cp (cpInv 2 (cpInv y seed1))) as [x z] eqn: H_OBS.
+      rewrite cp_spec in H_OBS. apply cpInv_inj in H_OBS. destruct H_OBS as [<- <-].
+      destruct (cp (cpInv y seed1)) as [x z] eqn: H_OBS. rewrite cp_spec in H_OBS. apply cpInv_inj in H_OBS. destruct H_OBS as [<- <-]. congruence.
+Qed.
+
+Theorem enum_frm_spec (p : frm)
+  : { x : nat | enum_frm x = p }.
+Proof.
+  epose proof (gen_frm_spec p (frm_depth p) _) as [seed H_EQ].
+  exists (cpInv (frm_depth p) seed). unfold enum_frm. destruct (cp (cpInv (frm_depth p) seed)) as [x y] eqn: H_OBS.
+  rewrite cp_spec in H_OBS. apply cpInv_inj in H_OBS. destruct H_OBS as [<- <-]. simpl. done.
+  Unshelve. reflexivity.
+Qed.
+
 End PROOF2.
 
 End ENUMERATION.
+
+Section INSTANCES.
+
+Context `(function_symbols_isEnumerable : isEnumerable L.(function_symbols)) `(constant_symbols_isEnumerable : isEnumerable L.(constant_symbols)).
+
+#[local]
+Instance trm_isEnumerable : isEnumerable trm :=
+  { enum := enum_trm function_symbols_isEnumerable.(enum) constant_symbols_isEnumerable.(enum)
+  ; enumerable := enum_trm_spec function_symbols_isEnumerable.(enum) constant_symbols_isEnumerable.(enum) function_symbols_isEnumerable.(enumerable) constant_symbols_isEnumerable.(enumerable)
+  }.
+
+#[local]
+Instance trms_isEnumerable (n : arity) : isEnumerable (trms n) :=
+  { enum := enum_trms function_symbols_isEnumerable.(enum) constant_symbols_isEnumerable.(enum)
+  ; enumerable := enum_trms_spec function_symbols_isEnumerable.(enum) constant_symbols_isEnumerable.(enum) function_symbols_isEnumerable.(enumerable) constant_symbols_isEnumerable.(enumerable) n
+  }.
+
+Context `(relation_symbols_isEnumerable : isEnumerable L.(relation_symbols)).
+
+#[local]
+Instance frms_isEnumerable : isEnumerable frm :=
+  { enum := enum_frm function_symbols_isEnumerable.(enum) constant_symbols_isEnumerable.(enum) relation_symbols_isEnumerable.(enum)
+  ; enumerable := enum_frm_spec function_symbols_isEnumerable.(enum) constant_symbols_isEnumerable.(enum) relation_symbols_isEnumerable.(enum) function_symbols_isEnumerable.(enumerable) constant_symbols_isEnumerable.(enumerable) relation_symbols_isEnumerable.(enumerable)
+  }.
+
+End INSTANCES.
 
 End SYNTAX.
 
